Summation.thy
@@ -110,7 +110,38 @@ lemma indexed_sum1_succ:
         (successor \<times>\<^sub>f id(\<nat>\<^sub>c\<^bsup>(\<nat>\<^sub>c \<times>\<^sub>c \<nat>\<^sub>c\<^bsup>\<nat>\<^sub>c\<^esup>)\<^esup>))\<rangle> \<circ>\<^sub>c indexed_sum1"
 by (typecheck_cfuncs, smt indexed_sum1_def2)
 
-
+lemma left_proj_index_sum1_id:
+  "left_cart_proj \<nat>\<^sub>c (\<nat>\<^sub>c\<^bsup>(\<nat>\<^sub>c \<times>\<^sub>c \<nat>\<^sub>c\<^bsup>\<nat>\<^sub>c\<^esup>)\<^esup>) \<circ>\<^sub>c indexed_sum1 = id \<nat>\<^sub>c"
+proof(etcs_rule natural_number_object_func_unique[where f = successor])
+  show "(left_cart_proj \<nat>\<^sub>c (\<nat>\<^sub>c\<^bsup>(\<nat>\<^sub>c \<times>\<^sub>c \<nat>\<^sub>c\<^bsup>\<nat>\<^sub>c\<^esup>)\<^esup>) \<circ>\<^sub>c indexed_sum1) \<circ>\<^sub>c zero = id\<^sub>c \<nat>\<^sub>c \<circ>\<^sub>c zero"
+    by(etcs_assocr, typecheck_cfuncs, smt (verit, best) comp_type eval_func_type id_left_unit2
+           indexed_sum1_zero left_cart_proj_cfunc_prod left_cart_proj_type transpose_func_type)
+  show "id\<^sub>c \<nat>\<^sub>c \<circ>\<^sub>c successor = successor \<circ>\<^sub>c id\<^sub>c \<nat>\<^sub>c"
+    by (typecheck_cfuncs, simp add: id_left_unit2 id_right_unit2)
+  show "(left_cart_proj \<nat>\<^sub>c (\<nat>\<^sub>c\<^bsup>(\<nat>\<^sub>c \<times>\<^sub>c \<nat>\<^sub>c\<^bsup>\<nat>\<^sub>c\<^esup>)\<^esup>) \<circ>\<^sub>c indexed_sum1) \<circ>\<^sub>c successor =
+    successor \<circ>\<^sub>c left_cart_proj \<nat>\<^sub>c (\<nat>\<^sub>c\<^bsup>(\<nat>\<^sub>c \<times>\<^sub>c \<nat>\<^sub>c\<^bsup>\<nat>\<^sub>c\<^esup>)\<^esup>) \<circ>\<^sub>c indexed_sum1"
+  proof -
+    have "(left_cart_proj \<nat>\<^sub>c (\<nat>\<^sub>c\<^bsup>(\<nat>\<^sub>c \<times>\<^sub>c \<nat>\<^sub>c\<^bsup>\<nat>\<^sub>c\<^esup>)\<^esup>) \<circ>\<^sub>c indexed_sum1) \<circ>\<^sub>c successor = 
+           left_cart_proj \<nat>\<^sub>c (\<nat>\<^sub>c\<^bsup>(\<nat>\<^sub>c \<times>\<^sub>c \<nat>\<^sub>c\<^bsup>\<nat>\<^sub>c\<^esup>)\<^esup>) \<circ>\<^sub>c indexed_sum1  \<circ>\<^sub>c successor"
+      by (etcs_assocl, simp)
+    also have "... = left_cart_proj \<nat>\<^sub>c (\<nat>\<^sub>c\<^bsup>(\<nat>\<^sub>c \<times>\<^sub>c \<nat>\<^sub>c\<^bsup>\<nat>\<^sub>c\<^esup>)\<^esup>) \<circ>\<^sub>c \<langle>successor \<circ>\<^sub>c left_cart_proj \<nat>\<^sub>c (\<nat>\<^sub>c\<^bsup>(\<nat>\<^sub>c \<times>\<^sub>c \<nat>\<^sub>c\<^bsup>\<nat>\<^sub>c\<^esup>)\<^esup>),
+        (add2 \<circ>\<^sub>c \<langle>eval_func  \<nat>\<^sub>c (\<nat>\<^sub>c \<times>\<^sub>c \<nat>\<^sub>c\<^bsup>\<nat>\<^sub>c\<^esup>) 
+              \<circ>\<^sub>c \<langle>left_cart_proj (\<nat>\<^sub>c \<times>\<^sub>c \<nat>\<^sub>c\<^bsup>\<nat>\<^sub>c\<^esup>) (\<nat>\<^sub>c \<times>\<^sub>c \<nat>\<^sub>c\<^bsup>(\<nat>\<^sub>c \<times>\<^sub>c \<nat>\<^sub>c\<^bsup>\<nat>\<^sub>c\<^esup>)\<^esup>),
+                    right_cart_proj \<nat>\<^sub>c (\<nat>\<^sub>c\<^bsup>(\<nat>\<^sub>c \<times>\<^sub>c \<nat>\<^sub>c\<^bsup>\<nat>\<^sub>c\<^esup>)\<^esup>)  \<circ>\<^sub>c 
+                    right_cart_proj (\<nat>\<^sub>c \<times>\<^sub>c \<nat>\<^sub>c\<^bsup>\<nat>\<^sub>c\<^esup>) (\<nat>\<^sub>c \<times>\<^sub>c \<nat>\<^sub>c\<^bsup>(\<nat>\<^sub>c \<times>\<^sub>c \<nat>\<^sub>c\<^bsup>\<nat>\<^sub>c\<^esup>)\<^esup>)\<rangle>,
+                  eval_func \<nat>\<^sub>c \<nat>\<^sub>c \<circ>\<^sub>c \<langle>add2 \<circ>\<^sub>c \<langle>left_cart_proj \<nat>\<^sub>c (\<nat>\<^sub>c\<^bsup>\<nat>\<^sub>c\<^esup>) \<circ>\<^sub>c 
+                  left_cart_proj (\<nat>\<^sub>c \<times>\<^sub>c \<nat>\<^sub>c\<^bsup>\<nat>\<^sub>c\<^esup>) (\<nat>\<^sub>c \<times>\<^sub>c \<nat>\<^sub>c\<^bsup>(\<nat>\<^sub>c \<times>\<^sub>c \<nat>\<^sub>c\<^bsup>\<nat>\<^sub>c\<^esup>)\<^esup>),
+                    left_cart_proj \<nat>\<^sub>c (\<nat>\<^sub>c\<^bsup>(\<nat>\<^sub>c \<times>\<^sub>c \<nat>\<^sub>c\<^bsup>\<nat>\<^sub>c\<^esup>)\<^esup>) \<circ>\<^sub>c 
+                    right_cart_proj (\<nat>\<^sub>c \<times>\<^sub>c \<nat>\<^sub>c\<^bsup>\<nat>\<^sub>c\<^esup>) (\<nat>\<^sub>c \<times>\<^sub>c \<nat>\<^sub>c\<^bsup>(\<nat>\<^sub>c \<times>\<^sub>c \<nat>\<^sub>c\<^bsup>\<nat>\<^sub>c\<^esup>)\<^esup>)\<rangle>,
+                  right_cart_proj \<nat>\<^sub>c (\<nat>\<^sub>c\<^bsup>\<nat>\<^sub>c\<^esup>) \<circ>\<^sub>c left_cart_proj (\<nat>\<^sub>c \<times>\<^sub>c \<nat>\<^sub>c\<^bsup>\<nat>\<^sub>c\<^esup>) (\<nat>\<^sub>c \<times>\<^sub>c \<nat>\<^sub>c\<^bsup>(\<nat>\<^sub>c \<times>\<^sub>c \<nat>\<^sub>c\<^bsup>\<nat>\<^sub>c\<^esup>)\<^esup>)\<rangle>\<rangle>)\<^sup>\<sharp> \<circ>\<^sub>c
+        (successor \<times>\<^sub>f id(\<nat>\<^sub>c\<^bsup>(\<nat>\<^sub>c \<times>\<^sub>c \<nat>\<^sub>c\<^bsup>\<nat>\<^sub>c\<^esup>)\<^esup>))\<rangle> \<circ>\<^sub>c indexed_sum1"
+      using indexed_sum1_succ by argo
+    also have "... = successor \<circ>\<^sub>c left_cart_proj \<nat>\<^sub>c (\<nat>\<^sub>c\<^bsup>(\<nat>\<^sub>c \<times>\<^sub>c \<nat>\<^sub>c\<^bsup>\<nat>\<^sub>c\<^esup>)\<^esup>)  \<circ>\<^sub>c indexed_sum1"
+      using left_cart_proj_cfunc_prod by(etcs_assocl,typecheck_cfuncs, auto)
+    then show ?thesis 
+      using calculation by auto
+  qed
+qed
 
 definition indexed_sum :: cfunc where
   "indexed_sum  = (right_cart_proj \<nat>\<^sub>c  (\<nat>\<^sub>c\<^bsup>(\<nat>\<^sub>c \<times>\<^sub>c \<nat>\<^sub>c\<^bsup>\<nat>\<^sub>c\<^esup>)\<^esup>) \<circ>\<^sub>c indexed_sum1)\<^sup>\<flat>"
@@ -150,12 +181,11 @@ proof (unfold indexed_sum_def)
     using calculation by auto
 qed
 
-
 lemma indexed_sum_tail_term:
   assumes "n \<in>\<^sub>c \<nat>\<^sub>c"
   assumes "m \<in>\<^sub>c \<nat>\<^sub>c"
   assumes "f \<in>\<^sub>c \<nat>\<^sub>c\<^bsup>\<nat>\<^sub>c\<^esup>"
-  shows "indexed_sum \<circ>\<^sub>c \<langle>\<langle>n, f\<rangle>, successor \<circ>\<^sub>c m\<rangle> =   indexed_sum \<circ>\<^sub>c \<langle>\<langle>n, f\<rangle>, m\<rangle> +\<^sub>\<nat> (cnufatem f \<circ>\<^sub>c successor \<circ>\<^sub>c m)"
+  shows "indexed_sum \<circ>\<^sub>c \<langle>\<langle>n, f\<rangle>, successor \<circ>\<^sub>c m\<rangle> = (indexed_sum \<circ>\<^sub>c \<langle>\<langle>n, f\<rangle>, m\<rangle>) +\<^sub>\<nat> (cnufatem f \<circ>\<^sub>c (n +\<^sub>\<nat> (successor \<circ>\<^sub>c m)))"
 proof (unfold indexed_sum_def)
   define \<phi> where "\<phi> = add2 \<circ>\<^sub>c \<langle>eval_func  \<nat>\<^sub>c (\<nat>\<^sub>c \<times>\<^sub>c \<nat>\<^sub>c\<^bsup>\<nat>\<^sub>c\<^esup>) 
               \<circ>\<^sub>c \<langle>left_cart_proj (\<nat>\<^sub>c \<times>\<^sub>c \<nat>\<^sub>c\<^bsup>\<nat>\<^sub>c\<^esup>) (\<nat>\<^sub>c \<times>\<^sub>c \<nat>\<^sub>c\<^bsup>(\<nat>\<^sub>c \<times>\<^sub>c \<nat>\<^sub>c\<^bsup>\<nat>\<^sub>c\<^esup>)\<^esup>),
@@ -211,28 +241,23 @@ proof (unfold indexed_sum_def)
               \<circ>\<^sub>c    \<langle>left_cart_proj (\<nat>\<^sub>c \<times>\<^sub>c \<nat>\<^sub>c\<^bsup>\<nat>\<^sub>c\<^esup>) (\<nat>\<^sub>c \<times>\<^sub>c \<nat>\<^sub>c\<^bsup>(\<nat>\<^sub>c \<times>\<^sub>c \<nat>\<^sub>c\<^bsup>\<nat>\<^sub>c\<^esup>)\<^esup>),
                     right_cart_proj \<nat>\<^sub>c (\<nat>\<^sub>c\<^bsup>(\<nat>\<^sub>c \<times>\<^sub>c \<nat>\<^sub>c\<^bsup>\<nat>\<^sub>c\<^esup>)\<^esup>)  \<circ>\<^sub>c 
                     right_cart_proj (\<nat>\<^sub>c \<times>\<^sub>c \<nat>\<^sub>c\<^bsup>\<nat>\<^sub>c\<^esup>) (\<nat>\<^sub>c \<times>\<^sub>c \<nat>\<^sub>c\<^bsup>(\<nat>\<^sub>c \<times>\<^sub>c \<nat>\<^sub>c\<^bsup>\<nat>\<^sub>c\<^esup>)\<^esup>)\<rangle>
-        \<circ>\<^sub>c \<langle>\<langle>n,f\<rangle>,(successor \<times>\<^sub>f id(\<nat>\<^sub>c\<^bsup>(\<nat>\<^sub>c \<times>\<^sub>c \<nat>\<^sub>c\<^bsup>\<nat>\<^sub>c\<^esup>)\<^esup>)) \<circ>\<^sub>c indexed_sum1 \<circ>\<^sub>c m\<rangle>
-                    ,
+        \<circ>\<^sub>c \<langle>\<langle>n,f\<rangle>,(successor \<times>\<^sub>f id(\<nat>\<^sub>c\<^bsup>(\<nat>\<^sub>c \<times>\<^sub>c \<nat>\<^sub>c\<^bsup>\<nat>\<^sub>c\<^esup>)\<^esup>)) \<circ>\<^sub>c indexed_sum1 \<circ>\<^sub>c m\<rangle>,
         eval_func \<nat>\<^sub>c \<nat>\<^sub>c \<circ>\<^sub>c 
                           \<langle>add2 \<circ>\<^sub>c 
                     \<langle>left_cart_proj \<nat>\<^sub>c (\<nat>\<^sub>c\<^bsup>\<nat>\<^sub>c\<^esup>) \<circ>\<^sub>c left_cart_proj (\<nat>\<^sub>c \<times>\<^sub>c \<nat>\<^sub>c\<^bsup>\<nat>\<^sub>c\<^esup>) (\<nat>\<^sub>c \<times>\<^sub>c \<nat>\<^sub>c\<^bsup>(\<nat>\<^sub>c \<times>\<^sub>c \<nat>\<^sub>c\<^bsup>\<nat>\<^sub>c\<^esup>)\<^esup>),
-                    left_cart_proj \<nat>\<^sub>c (\<nat>\<^sub>c\<^bsup>(\<nat>\<^sub>c \<times>\<^sub>c \<nat>\<^sub>c\<^bsup>\<nat>\<^sub>c\<^esup>)\<^esup>) \<circ>\<^sub>c right_cart_proj (\<nat>\<^sub>c \<times>\<^sub>c \<nat>\<^sub>c\<^bsup>\<nat>\<^sub>c\<^esup>) (\<nat>\<^sub>c \<times>\<^sub>c \<nat>\<^sub>c\<^bsup>(\<nat>\<^sub>c \<times>\<^sub>c \<nat>\<^sub>c\<^bsup>\<nat>\<^sub>c\<^esup>)\<^esup>)\<rangle>
-                          ,
+                    left_cart_proj \<nat>\<^sub>c (\<nat>\<^sub>c\<^bsup>(\<nat>\<^sub>c \<times>\<^sub>c \<nat>\<^sub>c\<^bsup>\<nat>\<^sub>c\<^esup>)\<^esup>) \<circ>\<^sub>c right_cart_proj (\<nat>\<^sub>c \<times>\<^sub>c \<nat>\<^sub>c\<^bsup>\<nat>\<^sub>c\<^esup>) (\<nat>\<^sub>c \<times>\<^sub>c \<nat>\<^sub>c\<^bsup>(\<nat>\<^sub>c \<times>\<^sub>c \<nat>\<^sub>c\<^bsup>\<nat>\<^sub>c\<^esup>)\<^esup>)\<rangle>,
               right_cart_proj \<nat>\<^sub>c (\<nat>\<^sub>c\<^bsup>\<nat>\<^sub>c\<^esup>) \<circ>\<^sub>c left_cart_proj (\<nat>\<^sub>c \<times>\<^sub>c \<nat>\<^sub>c\<^bsup>\<nat>\<^sub>c\<^esup>) (\<nat>\<^sub>c \<times>\<^sub>c \<nat>\<^sub>c\<^bsup>(\<nat>\<^sub>c \<times>\<^sub>c \<nat>\<^sub>c\<^bsup>\<nat>\<^sub>c\<^esup>)\<^esup>)\<rangle>
-        \<circ>\<^sub>c \<langle>\<langle>n,f\<rangle>,(successor \<times>\<^sub>f id(\<nat>\<^sub>c\<^bsup>(\<nat>\<^sub>c \<times>\<^sub>c \<nat>\<^sub>c\<^bsup>\<nat>\<^sub>c\<^esup>)\<^esup>)) \<circ>\<^sub>c indexed_sum1 \<circ>\<^sub>c m\<rangle> 
-        \<rangle>
-                  "
+        \<circ>\<^sub>c \<langle>\<langle>n,f\<rangle>,(successor \<times>\<^sub>f id(\<nat>\<^sub>c\<^bsup>(\<nat>\<^sub>c \<times>\<^sub>c \<nat>\<^sub>c\<^bsup>\<nat>\<^sub>c\<^esup>)\<^esup>)) \<circ>\<^sub>c indexed_sum1 \<circ>\<^sub>c m\<rangle>\<rangle>"
     using assms by (typecheck_cfuncs, smt (verit, best) cfunc_prod_comp comp_associative2)
   also have "... = (eval_func  \<nat>\<^sub>c (\<nat>\<^sub>c \<times>\<^sub>c \<nat>\<^sub>c\<^bsup>\<nat>\<^sub>c\<^esup>) 
               \<circ>\<^sub>c    \<langle>left_cart_proj (\<nat>\<^sub>c \<times>\<^sub>c \<nat>\<^sub>c\<^bsup>\<nat>\<^sub>c\<^esup>) (\<nat>\<^sub>c \<times>\<^sub>c \<nat>\<^sub>c\<^bsup>(\<nat>\<^sub>c \<times>\<^sub>c \<nat>\<^sub>c\<^bsup>\<nat>\<^sub>c\<^esup>)\<^esup>),
                     right_cart_proj \<nat>\<^sub>c (\<nat>\<^sub>c\<^bsup>(\<nat>\<^sub>c \<times>\<^sub>c \<nat>\<^sub>c\<^bsup>\<nat>\<^sub>c\<^esup>)\<^esup>)  \<circ>\<^sub>c 
                     right_cart_proj (\<nat>\<^sub>c \<times>\<^sub>c \<nat>\<^sub>c\<^bsup>\<nat>\<^sub>c\<^esup>) (\<nat>\<^sub>c \<times>\<^sub>c \<nat>\<^sub>c\<^bsup>(\<nat>\<^sub>c \<times>\<^sub>c \<nat>\<^sub>c\<^bsup>\<nat>\<^sub>c\<^esup>)\<^esup>)\<rangle>
-        \<circ>\<^sub>c \<langle>\<langle>n,f\<rangle>,(successor \<times>\<^sub>f id(\<nat>\<^sub>c\<^bsup>(\<nat>\<^sub>c \<times>\<^sub>c \<nat>\<^sub>c\<^bsup>\<nat>\<^sub>c\<^esup>)\<^esup>)) \<circ>\<^sub>c indexed_sum1 \<circ>\<^sub>c m\<rangle> )  +\<^sub>\<nat>
+        \<circ>\<^sub>c \<langle>\<langle>n,f\<rangle>,(successor \<times>\<^sub>f id(\<nat>\<^sub>c\<^bsup>(\<nat>\<^sub>c \<times>\<^sub>c \<nat>\<^sub>c\<^bsup>\<nat>\<^sub>c\<^esup>)\<^esup>)) \<circ>\<^sub>c indexed_sum1 \<circ>\<^sub>c m\<rangle>)  +\<^sub>\<nat>
        (eval_func \<nat>\<^sub>c \<nat>\<^sub>c \<circ>\<^sub>c 
                           \<langle>add2 \<circ>\<^sub>c 
                     \<langle>left_cart_proj \<nat>\<^sub>c (\<nat>\<^sub>c\<^bsup>\<nat>\<^sub>c\<^esup>) \<circ>\<^sub>c left_cart_proj (\<nat>\<^sub>c \<times>\<^sub>c \<nat>\<^sub>c\<^bsup>\<nat>\<^sub>c\<^esup>) (\<nat>\<^sub>c \<times>\<^sub>c \<nat>\<^sub>c\<^bsup>(\<nat>\<^sub>c \<times>\<^sub>c \<nat>\<^sub>c\<^bsup>\<nat>\<^sub>c\<^esup>)\<^esup>),
-                    left_cart_proj \<nat>\<^sub>c (\<nat>\<^sub>c\<^bsup>(\<nat>\<^sub>c \<times>\<^sub>c \<nat>\<^sub>c\<^bsup>\<nat>\<^sub>c\<^esup>)\<^esup>) \<circ>\<^sub>c right_cart_proj (\<nat>\<^sub>c \<times>\<^sub>c \<nat>\<^sub>c\<^bsup>\<nat>\<^sub>c\<^esup>) (\<nat>\<^sub>c \<times>\<^sub>c \<nat>\<^sub>c\<^bsup>(\<nat>\<^sub>c \<times>\<^sub>c \<nat>\<^sub>c\<^bsup>\<nat>\<^sub>c\<^esup>)\<^esup>)\<rangle>
-                          ,
+                    left_cart_proj \<nat>\<^sub>c (\<nat>\<^sub>c\<^bsup>(\<nat>\<^sub>c \<times>\<^sub>c \<nat>\<^sub>c\<^bsup>\<nat>\<^sub>c\<^esup>)\<^esup>) \<circ>\<^sub>c right_cart_proj (\<nat>\<^sub>c \<times>\<^sub>c \<nat>\<^sub>c\<^bsup>\<nat>\<^sub>c\<^esup>) (\<nat>\<^sub>c \<times>\<^sub>c \<nat>\<^sub>c\<^bsup>(\<nat>\<^sub>c \<times>\<^sub>c \<nat>\<^sub>c\<^bsup>\<nat>\<^sub>c\<^esup>)\<^esup>)\<rangle>,
               right_cart_proj \<nat>\<^sub>c (\<nat>\<^sub>c\<^bsup>\<nat>\<^sub>c\<^esup>) \<circ>\<^sub>c left_cart_proj (\<nat>\<^sub>c \<times>\<^sub>c \<nat>\<^sub>c\<^bsup>\<nat>\<^sub>c\<^esup>) (\<nat>\<^sub>c \<times>\<^sub>c \<nat>\<^sub>c\<^bsup>(\<nat>\<^sub>c \<times>\<^sub>c \<nat>\<^sub>c\<^bsup>\<nat>\<^sub>c\<^esup>)\<^esup>)\<rangle>
         \<circ>\<^sub>c \<langle>\<langle>n,f\<rangle>,(successor \<times>\<^sub>f id(\<nat>\<^sub>c\<^bsup>(\<nat>\<^sub>c \<times>\<^sub>c \<nat>\<^sub>c\<^bsup>\<nat>\<^sub>c\<^esup>)\<^esup>)) \<circ>\<^sub>c indexed_sum1 \<circ>\<^sub>c m\<rangle>)"
     using assms add_def by presburger
@@ -240,18 +265,211 @@ proof (unfold indexed_sum_def)
               \<circ>\<^sub>c    \<langle>left_cart_proj (\<nat>\<^sub>c \<times>\<^sub>c \<nat>\<^sub>c\<^bsup>\<nat>\<^sub>c\<^esup>) (\<nat>\<^sub>c \<times>\<^sub>c \<nat>\<^sub>c\<^bsup>(\<nat>\<^sub>c \<times>\<^sub>c \<nat>\<^sub>c\<^bsup>\<nat>\<^sub>c\<^esup>)\<^esup>),
                     right_cart_proj \<nat>\<^sub>c (\<nat>\<^sub>c\<^bsup>(\<nat>\<^sub>c \<times>\<^sub>c \<nat>\<^sub>c\<^bsup>\<nat>\<^sub>c\<^esup>)\<^esup>)  \<circ>\<^sub>c 
                     right_cart_proj (\<nat>\<^sub>c \<times>\<^sub>c \<nat>\<^sub>c\<^bsup>\<nat>\<^sub>c\<^esup>) (\<nat>\<^sub>c \<times>\<^sub>c \<nat>\<^sub>c\<^bsup>(\<nat>\<^sub>c \<times>\<^sub>c \<nat>\<^sub>c\<^bsup>\<nat>\<^sub>c\<^esup>)\<^esup>)\<rangle>
-        \<circ>\<^sub>c \<langle>\<langle>n,f\<rangle>,(successor \<times>\<^sub>f id(\<nat>\<^sub>c\<^bsup>(\<nat>\<^sub>c \<times>\<^sub>c \<nat>\<^sub>c\<^bsup>\<nat>\<^sub>c\<^esup>)\<^esup>)) \<circ>\<^sub>c indexed_sum1 \<circ>\<^sub>c m\<rangle> ) 
+        \<circ>\<^sub>c \<langle>\<langle>n,f\<rangle>,(successor \<times>\<^sub>f id(\<nat>\<^sub>c\<^bsup>(\<nat>\<^sub>c \<times>\<^sub>c \<nat>\<^sub>c\<^bsup>\<nat>\<^sub>c\<^esup>)\<^esup>)) \<circ>\<^sub>c indexed_sum1 \<circ>\<^sub>c m\<rangle>)  +\<^sub>\<nat>
+                   (eval_func \<nat>\<^sub>c \<nat>\<^sub>c \<circ>\<^sub>c 
+                        \<langle>add2 \<circ>\<^sub>c
+                        \<langle>left_cart_proj \<nat>\<^sub>c (\<nat>\<^sub>c\<^bsup>\<nat>\<^sub>c\<^esup>) \<circ>\<^sub>c left_cart_proj (\<nat>\<^sub>c \<times>\<^sub>c \<nat>\<^sub>c\<^bsup>\<nat>\<^sub>c\<^esup>) (\<nat>\<^sub>c \<times>\<^sub>c \<nat>\<^sub>c\<^bsup>(\<nat>\<^sub>c \<times>\<^sub>c \<nat>\<^sub>c\<^bsup>\<nat>\<^sub>c\<^esup>)\<^esup>),
+                         left_cart_proj \<nat>\<^sub>c (\<nat>\<^sub>c\<^bsup>(\<nat>\<^sub>c \<times>\<^sub>c \<nat>\<^sub>c\<^bsup>\<nat>\<^sub>c\<^esup>)\<^esup>) \<circ>\<^sub>c right_cart_proj (\<nat>\<^sub>c \<times>\<^sub>c \<nat>\<^sub>c\<^bsup>\<nat>\<^sub>c\<^esup>) (\<nat>\<^sub>c \<times>\<^sub>c \<nat>\<^sub>c\<^bsup>(\<nat>\<^sub>c \<times>\<^sub>c \<nat>\<^sub>c\<^bsup>\<nat>\<^sub>c\<^esup>)\<^esup>)\<rangle>
+                \<circ>\<^sub>c \<langle>\<langle>n,f\<rangle>,(successor \<times>\<^sub>f id(\<nat>\<^sub>c\<^bsup>(\<nat>\<^sub>c \<times>\<^sub>c \<nat>\<^sub>c\<^bsup>\<nat>\<^sub>c\<^esup>)\<^esup>)) \<circ>\<^sub>c indexed_sum1 \<circ>\<^sub>c m\<rangle>,
+                          right_cart_proj \<nat>\<^sub>c (\<nat>\<^sub>c\<^bsup>\<nat>\<^sub>c\<^esup>) \<circ>\<^sub>c left_cart_proj (\<nat>\<^sub>c \<times>\<^sub>c \<nat>\<^sub>c\<^bsup>\<nat>\<^sub>c\<^esup>) (\<nat>\<^sub>c \<times>\<^sub>c \<nat>\<^sub>c\<^bsup>(\<nat>\<^sub>c \<times>\<^sub>c \<nat>\<^sub>c\<^bsup>\<nat>\<^sub>c\<^esup>)\<^esup>)
+                \<circ>\<^sub>c \<langle>\<langle>n,f\<rangle>,(successor \<times>\<^sub>f id(\<nat>\<^sub>c\<^bsup>(\<nat>\<^sub>c \<times>\<^sub>c \<nat>\<^sub>c\<^bsup>\<nat>\<^sub>c\<^esup>)\<^esup>)) \<circ>\<^sub>c indexed_sum1 \<circ>\<^sub>c m\<rangle>\<rangle>)"
+    using assms by (etcs_assocl, typecheck_cfuncs, smt (verit, best) cfunc_prod_comp comp_associative2)
+  also have "... = (eval_func  \<nat>\<^sub>c (\<nat>\<^sub>c \<times>\<^sub>c \<nat>\<^sub>c\<^bsup>\<nat>\<^sub>c\<^esup>) 
+              \<circ>\<^sub>c    \<langle>left_cart_proj (\<nat>\<^sub>c \<times>\<^sub>c \<nat>\<^sub>c\<^bsup>\<nat>\<^sub>c\<^esup>) (\<nat>\<^sub>c \<times>\<^sub>c \<nat>\<^sub>c\<^bsup>(\<nat>\<^sub>c \<times>\<^sub>c \<nat>\<^sub>c\<^bsup>\<nat>\<^sub>c\<^esup>)\<^esup>),
+                    right_cart_proj \<nat>\<^sub>c (\<nat>\<^sub>c\<^bsup>(\<nat>\<^sub>c \<times>\<^sub>c \<nat>\<^sub>c\<^bsup>\<nat>\<^sub>c\<^esup>)\<^esup>)  \<circ>\<^sub>c 
+                    right_cart_proj (\<nat>\<^sub>c \<times>\<^sub>c \<nat>\<^sub>c\<^bsup>\<nat>\<^sub>c\<^esup>) (\<nat>\<^sub>c \<times>\<^sub>c \<nat>\<^sub>c\<^bsup>(\<nat>\<^sub>c \<times>\<^sub>c \<nat>\<^sub>c\<^bsup>\<nat>\<^sub>c\<^esup>)\<^esup>)\<rangle>
+        \<circ>\<^sub>c \<langle>\<langle>n,f\<rangle>,(successor \<times>\<^sub>f id(\<nat>\<^sub>c\<^bsup>(\<nat>\<^sub>c \<times>\<^sub>c \<nat>\<^sub>c\<^bsup>\<nat>\<^sub>c\<^esup>)\<^esup>)) \<circ>\<^sub>c indexed_sum1 \<circ>\<^sub>c m\<rangle>) 
   +\<^sub>\<nat>
        (eval_func \<nat>\<^sub>c \<nat>\<^sub>c \<circ>\<^sub>c 
                           \<langle>add2 \<circ>\<^sub>c 
-                    \<langle>left_cart_proj \<nat>\<^sub>c (\<nat>\<^sub>c\<^bsup>\<nat>\<^sub>c\<^esup>) \<circ>\<^sub>c left_cart_proj (\<nat>\<^sub>c \<times>\<^sub>c \<nat>\<^sub>c\<^bsup>\<nat>\<^sub>c\<^esup>) (\<nat>\<^sub>c \<times>\<^sub>c \<nat>\<^sub>c\<^bsup>(\<nat>\<^sub>c \<times>\<^sub>c \<nat>\<^sub>c\<^bsup>\<nat>\<^sub>c\<^esup>)\<^esup>),
-                    left_cart_proj \<nat>\<^sub>c (\<nat>\<^sub>c\<^bsup>(\<nat>\<^sub>c \<times>\<^sub>c \<nat>\<^sub>c\<^bsup>\<nat>\<^sub>c\<^esup>)\<^esup>) \<circ>\<^sub>c right_cart_proj (\<nat>\<^sub>c \<times>\<^sub>c \<nat>\<^sub>c\<^bsup>\<nat>\<^sub>c\<^esup>) (\<nat>\<^sub>c \<times>\<^sub>c \<nat>\<^sub>c\<^bsup>(\<nat>\<^sub>c \<times>\<^sub>c \<nat>\<^sub>c\<^bsup>\<nat>\<^sub>c\<^esup>)\<^esup>)\<rangle>
-                          ,
-              right_cart_proj \<nat>\<^sub>c (\<nat>\<^sub>c\<^bsup>\<nat>\<^sub>c\<^esup>) \<circ>\<^sub>c left_cart_proj (\<nat>\<^sub>c \<times>\<^sub>c \<nat>\<^sub>c\<^bsup>\<nat>\<^sub>c\<^esup>) (\<nat>\<^sub>c \<times>\<^sub>c \<nat>\<^sub>c\<^bsup>(\<nat>\<^sub>c \<times>\<^sub>c \<nat>\<^sub>c\<^bsup>\<nat>\<^sub>c\<^esup>)\<^esup>)\<rangle>
-        \<circ>\<^sub>c \<langle>\<langle>n,f\<rangle>,(successor \<times>\<^sub>f id(\<nat>\<^sub>c\<^bsup>(\<nat>\<^sub>c \<times>\<^sub>c \<nat>\<^sub>c\<^bsup>\<nat>\<^sub>c\<^esup>)\<^esup>)) \<circ>\<^sub>c indexed_sum1 \<circ>\<^sub>c m\<rangle>)"
+                   \<langle>left_cart_proj \<nat>\<^sub>c (\<nat>\<^sub>c\<^bsup>\<nat>\<^sub>c\<^esup>) \<circ>\<^sub>c left_cart_proj (\<nat>\<^sub>c \<times>\<^sub>c \<nat>\<^sub>c\<^bsup>\<nat>\<^sub>c\<^esup>) (\<nat>\<^sub>c \<times>\<^sub>c \<nat>\<^sub>c\<^bsup>(\<nat>\<^sub>c \<times>\<^sub>c \<nat>\<^sub>c\<^bsup>\<nat>\<^sub>c\<^esup>)\<^esup>)\<circ>\<^sub>c \<langle>\<langle>n,f\<rangle>,
+                   (successor \<times>\<^sub>f id(\<nat>\<^sub>c\<^bsup>(\<nat>\<^sub>c \<times>\<^sub>c \<nat>\<^sub>c\<^bsup>\<nat>\<^sub>c\<^esup>)\<^esup>)) \<circ>\<^sub>c indexed_sum1 \<circ>\<^sub>c m\<rangle>,
+                    left_cart_proj \<nat>\<^sub>c (\<nat>\<^sub>c\<^bsup>(\<nat>\<^sub>c \<times>\<^sub>c \<nat>\<^sub>c\<^bsup>\<nat>\<^sub>c\<^esup>)\<^esup>) \<circ>\<^sub>c right_cart_proj (\<nat>\<^sub>c \<times>\<^sub>c \<nat>\<^sub>c\<^bsup>\<nat>\<^sub>c\<^esup>) (\<nat>\<^sub>c \<times>\<^sub>c \<nat>\<^sub>c\<^bsup>(\<nat>\<^sub>c \<times>\<^sub>c \<nat>\<^sub>c\<^bsup>\<nat>\<^sub>c\<^esup>)\<^esup>)
+\<circ>\<^sub>c \<langle>\<langle>n,f\<rangle>,(successor \<times>\<^sub>f id(\<nat>\<^sub>c\<^bsup>(\<nat>\<^sub>c \<times>\<^sub>c \<nat>\<^sub>c\<^bsup>\<nat>\<^sub>c\<^esup>)\<^esup>)) \<circ>\<^sub>c indexed_sum1 \<circ>\<^sub>c m\<rangle>\<rangle>,f\<rangle>)"
+    using assms by (etcs_assocl, typecheck_cfuncs, smt (verit, best) cfunc_prod_comp comp_associative2 left_cart_proj_cfunc_prod right_cart_proj_cfunc_prod)
+  also have "... = (eval_func  \<nat>\<^sub>c (\<nat>\<^sub>c \<times>\<^sub>c \<nat>\<^sub>c\<^bsup>\<nat>\<^sub>c\<^esup>) 
+              \<circ>\<^sub>c    \<langle>left_cart_proj (\<nat>\<^sub>c \<times>\<^sub>c \<nat>\<^sub>c\<^bsup>\<nat>\<^sub>c\<^esup>) (\<nat>\<^sub>c \<times>\<^sub>c \<nat>\<^sub>c\<^bsup>(\<nat>\<^sub>c \<times>\<^sub>c \<nat>\<^sub>c\<^bsup>\<nat>\<^sub>c\<^esup>)\<^esup>),
+                    right_cart_proj \<nat>\<^sub>c (\<nat>\<^sub>c\<^bsup>(\<nat>\<^sub>c \<times>\<^sub>c \<nat>\<^sub>c\<^bsup>\<nat>\<^sub>c\<^esup>)\<^esup>)  \<circ>\<^sub>c 
+                    right_cart_proj (\<nat>\<^sub>c \<times>\<^sub>c \<nat>\<^sub>c\<^bsup>\<nat>\<^sub>c\<^esup>) (\<nat>\<^sub>c \<times>\<^sub>c \<nat>\<^sub>c\<^bsup>(\<nat>\<^sub>c \<times>\<^sub>c \<nat>\<^sub>c\<^bsup>\<nat>\<^sub>c\<^esup>)\<^esup>)\<rangle>
+        \<circ>\<^sub>c \<langle>\<langle>n,f\<rangle>,(successor \<times>\<^sub>f id(\<nat>\<^sub>c\<^bsup>(\<nat>\<^sub>c \<times>\<^sub>c \<nat>\<^sub>c\<^bsup>\<nat>\<^sub>c\<^esup>)\<^esup>)) \<circ>\<^sub>c indexed_sum1 \<circ>\<^sub>c m\<rangle>) 
+  +\<^sub>\<nat>
+       (eval_func \<nat>\<^sub>c \<nat>\<^sub>c \<circ>\<^sub>c \<langle>add2 \<circ>\<^sub>c 
+                    \<langle>n,left_cart_proj \<nat>\<^sub>c (\<nat>\<^sub>c\<^bsup>(\<nat>\<^sub>c \<times>\<^sub>c \<nat>\<^sub>c\<^bsup>\<nat>\<^sub>c\<^esup>)\<^esup>) \<circ>\<^sub>c (successor \<times>\<^sub>f id(\<nat>\<^sub>c\<^bsup>(\<nat>\<^sub>c \<times>\<^sub>c \<nat>\<^sub>c\<^bsup>\<nat>\<^sub>c\<^esup>)\<^esup>)) \<circ>\<^sub>c indexed_sum1 \<circ>\<^sub>c m\<rangle>,f \<rangle>)"
+    using left_cart_proj_cfunc_prod right_cart_proj_cfunc_prod assms by (typecheck_cfuncs, auto)
+  also have "... = (eval_func  \<nat>\<^sub>c (\<nat>\<^sub>c \<times>\<^sub>c \<nat>\<^sub>c\<^bsup>\<nat>\<^sub>c\<^esup>) 
+              \<circ>\<^sub>c    \<langle>left_cart_proj (\<nat>\<^sub>c \<times>\<^sub>c \<nat>\<^sub>c\<^bsup>\<nat>\<^sub>c\<^esup>) (\<nat>\<^sub>c \<times>\<^sub>c \<nat>\<^sub>c\<^bsup>(\<nat>\<^sub>c \<times>\<^sub>c \<nat>\<^sub>c\<^bsup>\<nat>\<^sub>c\<^esup>)\<^esup>),
+                    right_cart_proj \<nat>\<^sub>c (\<nat>\<^sub>c\<^bsup>(\<nat>\<^sub>c \<times>\<^sub>c \<nat>\<^sub>c\<^bsup>\<nat>\<^sub>c\<^esup>)\<^esup>)  \<circ>\<^sub>c 
+                    right_cart_proj (\<nat>\<^sub>c \<times>\<^sub>c \<nat>\<^sub>c\<^bsup>\<nat>\<^sub>c\<^esup>) (\<nat>\<^sub>c \<times>\<^sub>c \<nat>\<^sub>c\<^bsup>(\<nat>\<^sub>c \<times>\<^sub>c \<nat>\<^sub>c\<^bsup>\<nat>\<^sub>c\<^esup>)\<^esup>)\<rangle>
+        \<circ>\<^sub>c \<langle>\<langle>n,f\<rangle>,(successor \<times>\<^sub>f id(\<nat>\<^sub>c\<^bsup>(\<nat>\<^sub>c \<times>\<^sub>c \<nat>\<^sub>c\<^bsup>\<nat>\<^sub>c\<^esup>)\<^esup>)) \<circ>\<^sub>c indexed_sum1 \<circ>\<^sub>c m\<rangle>) 
+  +\<^sub>\<nat>
+       (eval_func \<nat>\<^sub>c \<nat>\<^sub>c \<circ>\<^sub>c 
+                          \<langle>add2 \<circ>\<^sub>c 
+                    \<langle>n,  successor \<circ>\<^sub>c  left_cart_proj \<nat>\<^sub>c (\<nat>\<^sub>c\<^bsup>(\<nat>\<^sub>c \<times>\<^sub>c \<nat>\<^sub>c\<^bsup>\<nat>\<^sub>c\<^esup>)\<^esup>) \<circ>\<^sub>c indexed_sum1 \<circ>\<^sub>c m\<rangle>, f\<rangle>)"
+    using assms by (etcs_assocl, typecheck_cfuncs, smt (verit, best) left_cart_proj_cfunc_cross_prod)
+  also have "... = (eval_func  \<nat>\<^sub>c (\<nat>\<^sub>c \<times>\<^sub>c \<nat>\<^sub>c\<^bsup>\<nat>\<^sub>c\<^esup>) 
+              \<circ>\<^sub>c    \<langle>left_cart_proj (\<nat>\<^sub>c \<times>\<^sub>c \<nat>\<^sub>c\<^bsup>\<nat>\<^sub>c\<^esup>) (\<nat>\<^sub>c \<times>\<^sub>c \<nat>\<^sub>c\<^bsup>(\<nat>\<^sub>c \<times>\<^sub>c \<nat>\<^sub>c\<^bsup>\<nat>\<^sub>c\<^esup>)\<^esup>),
+                    right_cart_proj \<nat>\<^sub>c (\<nat>\<^sub>c\<^bsup>(\<nat>\<^sub>c \<times>\<^sub>c \<nat>\<^sub>c\<^bsup>\<nat>\<^sub>c\<^esup>)\<^esup>)  \<circ>\<^sub>c 
+                    right_cart_proj (\<nat>\<^sub>c \<times>\<^sub>c \<nat>\<^sub>c\<^bsup>\<nat>\<^sub>c\<^esup>) (\<nat>\<^sub>c \<times>\<^sub>c \<nat>\<^sub>c\<^bsup>(\<nat>\<^sub>c \<times>\<^sub>c \<nat>\<^sub>c\<^bsup>\<nat>\<^sub>c\<^esup>)\<^esup>)\<rangle>
+        \<circ>\<^sub>c \<langle>\<langle>n,f\<rangle>,(successor \<times>\<^sub>f id(\<nat>\<^sub>c\<^bsup>(\<nat>\<^sub>c \<times>\<^sub>c \<nat>\<^sub>c\<^bsup>\<nat>\<^sub>c\<^esup>)\<^esup>)) \<circ>\<^sub>c indexed_sum1 \<circ>\<^sub>c m\<rangle>) 
+  +\<^sub>\<nat>
+       (eval_func \<nat>\<^sub>c \<nat>\<^sub>c \<circ>\<^sub>c \<langle>add2 \<circ>\<^sub>c \<langle>n,  successor  \<circ>\<^sub>c m\<rangle>, f\<rangle>)"
+    using assms  by (etcs_assocl,etcs_assocr, typecheck_cfuncs, simp add: cfunc_type_def comp_associative id_left_unit2 left_proj_index_sum1_id)
+  also have "... = (eval_func  \<nat>\<^sub>c (\<nat>\<^sub>c \<times>\<^sub>c \<nat>\<^sub>c\<^bsup>\<nat>\<^sub>c\<^esup>) 
+              \<circ>\<^sub>c    \<langle>left_cart_proj (\<nat>\<^sub>c \<times>\<^sub>c \<nat>\<^sub>c\<^bsup>\<nat>\<^sub>c\<^esup>) (\<nat>\<^sub>c \<times>\<^sub>c \<nat>\<^sub>c\<^bsup>(\<nat>\<^sub>c \<times>\<^sub>c \<nat>\<^sub>c\<^bsup>\<nat>\<^sub>c\<^esup>)\<^esup>),
+                    right_cart_proj \<nat>\<^sub>c (\<nat>\<^sub>c\<^bsup>(\<nat>\<^sub>c \<times>\<^sub>c \<nat>\<^sub>c\<^bsup>\<nat>\<^sub>c\<^esup>)\<^esup>)  \<circ>\<^sub>c 
+                    right_cart_proj (\<nat>\<^sub>c \<times>\<^sub>c \<nat>\<^sub>c\<^bsup>\<nat>\<^sub>c\<^esup>) (\<nat>\<^sub>c \<times>\<^sub>c \<nat>\<^sub>c\<^bsup>(\<nat>\<^sub>c \<times>\<^sub>c \<nat>\<^sub>c\<^bsup>\<nat>\<^sub>c\<^esup>)\<^esup>)\<rangle>
+        \<circ>\<^sub>c \<langle>\<langle>n,f\<rangle>,(successor \<times>\<^sub>f id(\<nat>\<^sub>c\<^bsup>(\<nat>\<^sub>c \<times>\<^sub>c \<nat>\<^sub>c\<^bsup>\<nat>\<^sub>c\<^esup>)\<^esup>)) \<circ>\<^sub>c indexed_sum1 \<circ>\<^sub>c m\<rangle>) 
+  +\<^sub>\<nat>
+       (cnufatem f \<circ>\<^sub>c (n +\<^sub>\<nat> (successor \<circ>\<^sub>c m)))"
+    by (typecheck_cfuncs, metis add_def assms(1) assms(2) assms(3) eval_lemma metafunc_cnufatem)
+  also have "... = (eval_func  \<nat>\<^sub>c (\<nat>\<^sub>c \<times>\<^sub>c \<nat>\<^sub>c\<^bsup>\<nat>\<^sub>c\<^esup>) 
+              \<circ>\<^sub>c    \<langle>left_cart_proj (\<nat>\<^sub>c \<times>\<^sub>c \<nat>\<^sub>c\<^bsup>\<nat>\<^sub>c\<^esup>) (\<nat>\<^sub>c \<times>\<^sub>c \<nat>\<^sub>c\<^bsup>(\<nat>\<^sub>c \<times>\<^sub>c \<nat>\<^sub>c\<^bsup>\<nat>\<^sub>c\<^esup>)\<^esup>)
+    \<circ>\<^sub>c \<langle>\<langle>n,f\<rangle>,(successor \<times>\<^sub>f id(\<nat>\<^sub>c\<^bsup>(\<nat>\<^sub>c \<times>\<^sub>c \<nat>\<^sub>c\<^bsup>\<nat>\<^sub>c\<^esup>)\<^esup>)) \<circ>\<^sub>c indexed_sum1 \<circ>\<^sub>c m\<rangle>,
+                    right_cart_proj \<nat>\<^sub>c (\<nat>\<^sub>c\<^bsup>(\<nat>\<^sub>c \<times>\<^sub>c \<nat>\<^sub>c\<^bsup>\<nat>\<^sub>c\<^esup>)\<^esup>)  \<circ>\<^sub>c 
+                    right_cart_proj (\<nat>\<^sub>c \<times>\<^sub>c \<nat>\<^sub>c\<^bsup>\<nat>\<^sub>c\<^esup>) (\<nat>\<^sub>c \<times>\<^sub>c \<nat>\<^sub>c\<^bsup>(\<nat>\<^sub>c \<times>\<^sub>c \<nat>\<^sub>c\<^bsup>\<nat>\<^sub>c\<^esup>)\<^esup>) 
+    \<circ>\<^sub>c \<langle>\<langle>n,f\<rangle>,(successor \<times>\<^sub>f id(\<nat>\<^sub>c\<^bsup>(\<nat>\<^sub>c \<times>\<^sub>c \<nat>\<^sub>c\<^bsup>\<nat>\<^sub>c\<^esup>)\<^esup>)) \<circ>\<^sub>c indexed_sum1 \<circ>\<^sub>c m\<rangle>\<rangle>) 
+  +\<^sub>\<nat>
+       (cnufatem f \<circ>\<^sub>c (n +\<^sub>\<nat> (successor \<circ>\<^sub>c m)))"
+    using assms cfunc_prod_comp comp_associative2 by (typecheck_cfuncs, force)
+  also have "... = (eval_func  \<nat>\<^sub>c (\<nat>\<^sub>c \<times>\<^sub>c \<nat>\<^sub>c\<^bsup>\<nat>\<^sub>c\<^esup>) 
+              \<circ>\<^sub>c    \<langle>\<langle>n,f\<rangle>,
+                    right_cart_proj \<nat>\<^sub>c (\<nat>\<^sub>c\<^bsup>(\<nat>\<^sub>c \<times>\<^sub>c \<nat>\<^sub>c\<^bsup>\<nat>\<^sub>c\<^esup>)\<^esup>)  \<circ>\<^sub>c 
+                    right_cart_proj (\<nat>\<^sub>c \<times>\<^sub>c \<nat>\<^sub>c\<^bsup>\<nat>\<^sub>c\<^esup>) (\<nat>\<^sub>c \<times>\<^sub>c \<nat>\<^sub>c\<^bsup>(\<nat>\<^sub>c \<times>\<^sub>c \<nat>\<^sub>c\<^bsup>\<nat>\<^sub>c\<^esup>)\<^esup>) 
+    \<circ>\<^sub>c \<langle>\<langle>n,f\<rangle>,(successor \<times>\<^sub>f id(\<nat>\<^sub>c\<^bsup>(\<nat>\<^sub>c \<times>\<^sub>c \<nat>\<^sub>c\<^bsup>\<nat>\<^sub>c\<^esup>)\<^esup>)) \<circ>\<^sub>c indexed_sum1 \<circ>\<^sub>c m\<rangle>\<rangle>) 
+  +\<^sub>\<nat>
+       (cnufatem f \<circ>\<^sub>c (n +\<^sub>\<nat> (successor \<circ>\<^sub>c m)))"
+    using assms left_cart_proj_cfunc_prod by (typecheck_cfuncs, auto)
+  also have "... = (eval_func  \<nat>\<^sub>c (\<nat>\<^sub>c \<times>\<^sub>c \<nat>\<^sub>c\<^bsup>\<nat>\<^sub>c\<^esup>) \<circ>\<^sub>c \<langle>\<langle>n,f\<rangle>,  right_cart_proj \<nat>\<^sub>c (\<nat>\<^sub>c\<^bsup>(\<nat>\<^sub>c \<times>\<^sub>c \<nat>\<^sub>c\<^bsup>\<nat>\<^sub>c\<^esup>)\<^esup>)  \<circ>\<^sub>c              
+           (successor \<times>\<^sub>f id(\<nat>\<^sub>c\<^bsup>(\<nat>\<^sub>c \<times>\<^sub>c \<nat>\<^sub>c\<^bsup>\<nat>\<^sub>c\<^esup>)\<^esup>)) \<circ>\<^sub>c indexed_sum1 \<circ>\<^sub>c m\<rangle>) +\<^sub>\<nat>  (cnufatem f \<circ>\<^sub>c (n +\<^sub>\<nat> (successor \<circ>\<^sub>c m)))"
+    using assms right_cart_proj_cfunc_prod by (typecheck_cfuncs, auto)
+  also have "... = (eval_func  \<nat>\<^sub>c (\<nat>\<^sub>c \<times>\<^sub>c \<nat>\<^sub>c\<^bsup>\<nat>\<^sub>c\<^esup>) \<circ>\<^sub>c \<langle> \<langle>n,f\<rangle>,  id(\<nat>\<^sub>c\<^bsup>(\<nat>\<^sub>c \<times>\<^sub>c \<nat>\<^sub>c\<^bsup>\<nat>\<^sub>c\<^esup>)\<^esup>) \<circ>\<^sub>c
+                     right_cart_proj \<nat>\<^sub>c (\<nat>\<^sub>c\<^bsup>(\<nat>\<^sub>c \<times>\<^sub>c \<nat>\<^sub>c\<^bsup>\<nat>\<^sub>c\<^esup>)\<^esup>) \<circ>\<^sub>c indexed_sum1 \<circ>\<^sub>c m\<rangle>)   +\<^sub>\<nat>
+                           (cnufatem f \<circ>\<^sub>c (n +\<^sub>\<nat> (successor \<circ>\<^sub>c m)))"
+    using assms right_cart_proj_cfunc_cross_prod by(etcs_assocl, typecheck_cfuncs, auto)
+  also have "... = (eval_func  \<nat>\<^sub>c (\<nat>\<^sub>c \<times>\<^sub>c \<nat>\<^sub>c\<^bsup>\<nat>\<^sub>c\<^esup>) \<circ>\<^sub>c (id(\<nat>\<^sub>c \<times>\<^sub>c \<nat>\<^sub>c\<^bsup>\<nat>\<^sub>c\<^esup>) \<times>\<^sub>f (right_cart_proj \<nat>\<^sub>c (\<nat>\<^sub>c\<^bsup>(\<nat>\<^sub>c \<times>\<^sub>c \<nat>\<^sub>c\<^bsup>\<nat>\<^sub>c\<^esup>)\<^esup>)   \<circ>\<^sub>c indexed_sum1) ) \<circ>\<^sub>c  \<langle> \<langle>n,f\<rangle>,  m\<rangle>)          
+                        +\<^sub>\<nat> (cnufatem f \<circ>\<^sub>c (n +\<^sub>\<nat> (successor \<circ>\<^sub>c m)))"
+    using assms by(etcs_assocl, typecheck_cfuncs, smt (verit, best) cfunc_cross_prod_comp_cfunc_prod comp_associative2 id_left_unit2)
+  also have "... = ((right_cart_proj \<nat>\<^sub>c (\<nat>\<^sub>c\<^bsup>(\<nat>\<^sub>c \<times>\<^sub>c \<nat>\<^sub>c\<^bsup>\<nat>\<^sub>c\<^esup>)\<^esup>) \<circ>\<^sub>c indexed_sum1)\<^sup>\<flat> \<circ>\<^sub>c \<langle>\<langle>n,f\<rangle>,m\<rangle>) +\<^sub>\<nat> (cnufatem f \<circ>\<^sub>c (n +\<^sub>\<nat> (successor \<circ>\<^sub>c m)))"
+    using assms inv_transpose_func_def2 by (etcs_assocl, typecheck_cfuncs, auto)
+  then show "(right_cart_proj \<nat>\<^sub>c (\<nat>\<^sub>c\<^bsup>(\<nat>\<^sub>c \<times>\<^sub>c \<nat>\<^sub>c\<^bsup>\<nat>\<^sub>c\<^esup>)\<^esup>) \<circ>\<^sub>c indexed_sum1)\<^sup>\<flat> \<circ>\<^sub>c \<langle>\<langle>n,f\<rangle>,successor \<circ>\<^sub>c m\<rangle> =
+                    ((right_cart_proj \<nat>\<^sub>c (\<nat>\<^sub>c\<^bsup>(\<nat>\<^sub>c \<times>\<^sub>c \<nat>\<^sub>c\<^bsup>\<nat>\<^sub>c\<^esup>)\<^esup>) \<circ>\<^sub>c indexed_sum1)\<^sup>\<flat> \<circ>\<^sub>c \<langle>\<langle>n,f\<rangle>,m\<rangle>)  +\<^sub>\<nat> (cnufatem f \<circ>\<^sub>c (n +\<^sub>\<nat> (successor \<circ>\<^sub>c m)))"
+    using calculation by auto
+qed
+
+lemma sum_indexed_sum:
+  assumes "a \<in>\<^sub>c \<nat>\<^sub>c"
+  assumes "b \<in>\<^sub>c \<nat>\<^sub>c"
+  assumes "f \<in>\<^sub>c \<nat>\<^sub>c\<^bsup>\<nat>\<^sub>c\<^esup>"
+  assumes "g \<in>\<^sub>c \<nat>\<^sub>c\<^bsup>\<nat>\<^sub>c\<^esup>"
+  shows "indexed_sum \<circ>\<^sub>c \<langle>\<langle>a, meta_add \<nat>\<^sub>c \<circ>\<^sub>c \<langle>f,g\<rangle> \<rangle>, n \<rangle> = 
+          (indexed_sum \<circ>\<^sub>c \<langle>\<langle>a, f \<rangle>, n \<rangle>) +\<^sub>\<nat> (indexed_sum \<circ>\<^sub>c \<langle>\<langle>a, g \<rangle>, n \<rangle>)"
+proof(unfold meta_add_def indexed_sum_def)
+  have "(right_cart_proj \<nat>\<^sub>c (\<nat>\<^sub>c\<^bsup>(\<nat>\<^sub>c \<times>\<^sub>c \<nat>\<^sub>c\<^bsup>\<nat>\<^sub>c\<^esup>)\<^esup>) \<circ>\<^sub>c indexed_sum1)\<^sup>\<flat> \<circ>\<^sub>c
+    \<langle>\<langle>a,(add2 \<circ>\<^sub>c (eval_func \<nat>\<^sub>c \<nat>\<^sub>c \<times>\<^sub>f eval_func \<nat>\<^sub>c \<nat>\<^sub>c) \<circ>\<^sub>c distribute_left \<nat>\<^sub>c (\<nat>\<^sub>c\<^bsup>\<nat>\<^sub>c\<^esup>) (\<nat>\<^sub>c\<^bsup>\<nat>\<^sub>c\<^esup>))\<^sup>\<sharp> \<circ>\<^sub>c \<langle>f,g\<rangle>\<rangle>  \<circ>\<^sub>c \<beta>\<^bsub>\<nat>\<^sub>c\<^esub>,id \<nat>\<^sub>c\<rangle> = 
+   add2 \<circ>\<^sub>c \<langle> ((right_cart_proj \<nat>\<^sub>c (\<nat>\<^sub>c\<^bsup>(\<nat>\<^sub>c \<times>\<^sub>c \<nat>\<^sub>c\<^bsup>\<nat>\<^sub>c\<^esup>)\<^esup>) \<circ>\<^sub>c indexed_sum1)\<^sup>\<flat> \<circ>\<^sub>c \<langle>\<langle>a,f\<rangle> \<circ>\<^sub>c \<beta>\<^bsub>\<nat>\<^sub>c\<^esub>,id \<nat>\<^sub>c\<rangle>),
+    ((right_cart_proj \<nat>\<^sub>c (\<nat>\<^sub>c\<^bsup>(\<nat>\<^sub>c \<times>\<^sub>c \<nat>\<^sub>c\<^bsup>\<nat>\<^sub>c\<^esup>)\<^esup>) \<circ>\<^sub>c indexed_sum1)\<^sup>\<flat> \<circ>\<^sub>c \<langle>\<langle>a,g\<rangle> \<circ>\<^sub>c \<beta>\<^bsub>\<nat>\<^sub>c\<^esub>, id \<nat>\<^sub>c\<rangle>)\<rangle>"
+  proof(rule natural_number_object_func_unique[where X = "\<nat>\<^sub>c"])
+    show "(right_cart_proj \<nat>\<^sub>c (\<nat>\<^sub>c\<^bsup>(\<nat>\<^sub>c \<times>\<^sub>c \<nat>\<^sub>c\<^bsup>\<nat>\<^sub>c\<^esup>)\<^esup>) \<circ>\<^sub>c indexed_sum1)\<^sup>\<flat> \<circ>\<^sub>c
+    \<langle>\<langle>a,(add2 \<circ>\<^sub>c (eval_func \<nat>\<^sub>c \<nat>\<^sub>c \<times>\<^sub>f eval_func \<nat>\<^sub>c \<nat>\<^sub>c) \<circ>\<^sub>c distribute_left \<nat>\<^sub>c (\<nat>\<^sub>c\<^bsup>\<nat>\<^sub>c\<^esup>) (\<nat>\<^sub>c\<^bsup>\<nat>\<^sub>c\<^esup>))\<^sup>\<sharp> \<circ>\<^sub>c \<langle>f,g\<rangle>\<rangle> \<circ>\<^sub>c
+     \<beta>\<^bsub>\<nat>\<^sub>c\<^esub>,id\<^sub>c \<nat>\<^sub>c\<rangle> : \<nat>\<^sub>c \<rightarrow> \<nat>\<^sub>c"
+      using assms by typecheck_cfuncs 
+    show "add2 \<circ>\<^sub>c
+    \<langle>(right_cart_proj \<nat>\<^sub>c (\<nat>\<^sub>c\<^bsup>(\<nat>\<^sub>c \<times>\<^sub>c \<nat>\<^sub>c\<^bsup>\<nat>\<^sub>c\<^esup>)\<^esup>) \<circ>\<^sub>c indexed_sum1)\<^sup>\<flat> \<circ>\<^sub>c
+     \<langle>\<langle>a,f\<rangle> \<circ>\<^sub>c \<beta>\<^bsub>\<nat>\<^sub>c\<^esub>,id\<^sub>c \<nat>\<^sub>c\<rangle>,(right_cart_proj \<nat>\<^sub>c (\<nat>\<^sub>c\<^bsup>(\<nat>\<^sub>c \<times>\<^sub>c \<nat>\<^sub>c\<^bsup>\<nat>\<^sub>c\<^esup>)\<^esup>) \<circ>\<^sub>c indexed_sum1)\<^sup>\<flat> \<circ>\<^sub>c \<langle>\<langle>a,g\<rangle> \<circ>\<^sub>c \<beta>\<^bsub>\<nat>\<^sub>c\<^esub>,id\<^sub>c \<nat>\<^sub>c\<rangle>\<rangle> : \<nat>\<^sub>c \<rightarrow> \<nat>\<^sub>c"
+      using assms by typecheck_cfuncs
+  next
+
+(*
+    have "(add2 \<circ>\<^sub>c
+     \<langle>(right_cart_proj \<nat>\<^sub>c (\<nat>\<^sub>c\<^bsup>(\<nat>\<^sub>c \<times>\<^sub>c \<nat>\<^sub>c\<^bsup>\<nat>\<^sub>c\<^esup>)\<^esup>) \<circ>\<^sub>c indexed_sum1)\<^sup>\<flat> \<circ>\<^sub>c
+      \<langle>\<langle>a,f\<rangle> \<circ>\<^sub>c \<beta>\<^bsub>\<nat>\<^sub>c\<^esub>,id\<^sub>c \<nat>\<^sub>c\<rangle>,(right_cart_proj \<nat>\<^sub>c (\<nat>\<^sub>c\<^bsup>(\<nat>\<^sub>c \<times>\<^sub>c \<nat>\<^sub>c\<^bsup>\<nat>\<^sub>c\<^esup>)\<^esup>) \<circ>\<^sub>c indexed_sum1)\<^sup>\<flat> \<circ>\<^sub>c \<langle>\<langle>a,g\<rangle> \<circ>\<^sub>c \<beta>\<^bsub>\<nat>\<^sub>c\<^esub>,id\<^sub>c \<nat>\<^sub>c\<rangle>\<rangle>) \<circ>\<^sub>c
+    zero = add2 \<circ>\<^sub>c
+     \<langle>(right_cart_proj \<nat>\<^sub>c (\<nat>\<^sub>c\<^bsup>(\<nat>\<^sub>c \<times>\<^sub>c \<nat>\<^sub>c\<^bsup>\<nat>\<^sub>c\<^esup>)\<^esup>) \<circ>\<^sub>c indexed_sum1)\<^sup>\<flat> \<circ>\<^sub>c
+      \<langle>\<langle>a,f\<rangle>, zero\<rangle>,(right_cart_proj \<nat>\<^sub>c (\<nat>\<^sub>c\<^bsup>(\<nat>\<^sub>c \<times>\<^sub>c \<nat>\<^sub>c\<^bsup>\<nat>\<^sub>c\<^esup>)\<^esup>) \<circ>\<^sub>c indexed_sum1)\<^sup>\<flat> \<circ>\<^sub>c \<langle>\<langle>a,g\<rangle> ,zero\<rangle>\<rangle>"
+      using assms by (typecheck_cfuncs, smt (verit, ccfv_SIG) cfunc_prod_comp comp_associative2 left_param_def2 left_param_on_el)
+    also have "... =  ((right_cart_proj \<nat>\<^sub>c (\<nat>\<^sub>c\<^bsup>(\<nat>\<^sub>c \<times>\<^sub>c \<nat>\<^sub>c\<^bsup>\<nat>\<^sub>c\<^esup>)\<^esup>) \<circ>\<^sub>c indexed_sum1)\<^sup>\<flat> \<circ>\<^sub>c \<langle>\<langle>a,f\<rangle>, zero\<rangle>) +\<^sub>\<nat> 
+                      ((right_cart_proj \<nat>\<^sub>c (\<nat>\<^sub>c\<^bsup>(\<nat>\<^sub>c \<times>\<^sub>c \<nat>\<^sub>c\<^bsup>\<nat>\<^sub>c\<^esup>)\<^esup>) \<circ>\<^sub>c indexed_sum1)\<^sup>\<flat> \<circ>\<^sub>c \<langle>\<langle>a,g\<rangle> ,zero\<rangle>)"
+      using assms add_def by presburger
+    also have "... =  ((eval_func \<nat>\<^sub>c (\<nat>\<^sub>c \<times>\<^sub>c \<nat>\<^sub>c\<^bsup>\<nat>\<^sub>c\<^esup>)) \<circ>\<^sub>c (id (\<nat>\<^sub>c \<times>\<^sub>c (\<nat>\<^sub>c\<^bsup>\<nat>\<^sub>c\<^esup>)) \<times>\<^sub>f ((right_cart_proj \<nat>\<^sub>c (\<nat>\<^sub>c\<^bsup>(\<nat>\<^sub>c \<times>\<^sub>c \<nat>\<^sub>c\<^bsup>\<nat>\<^sub>c\<^esup>)\<^esup>)) \<circ>\<^sub>c indexed_sum1)) \<circ>\<^sub>c \<langle>\<langle>a,f\<rangle>, zero\<rangle>) +\<^sub>\<nat> 
+                      ((eval_func \<nat>\<^sub>c (\<nat>\<^sub>c \<times>\<^sub>c \<nat>\<^sub>c\<^bsup>\<nat>\<^sub>c\<^esup>)) \<circ>\<^sub>c (id (\<nat>\<^sub>c \<times>\<^sub>c (\<nat>\<^sub>c\<^bsup>\<nat>\<^sub>c\<^esup>)) \<times>\<^sub>f ((right_cart_proj \<nat>\<^sub>c (\<nat>\<^sub>c\<^bsup>(\<nat>\<^sub>c \<times>\<^sub>c \<nat>\<^sub>c\<^bsup>\<nat>\<^sub>c\<^esup>)\<^esup>)) \<circ>\<^sub>c indexed_sum1)) \<circ>\<^sub>c \<langle>\<langle>a,g\<rangle> ,zero\<rangle>)"
+      using assms comp_associative2 inv_transpose_func_def2 by (typecheck_cfuncs, force)
+    also have "... =  ((eval_func \<nat>\<^sub>c (\<nat>\<^sub>c \<times>\<^sub>c \<nat>\<^sub>c\<^bsup>\<nat>\<^sub>c\<^esup>)) \<circ>\<^sub>c (id (\<nat>\<^sub>c \<times>\<^sub>c (\<nat>\<^sub>c\<^bsup>\<nat>\<^sub>c\<^esup>)) \<times>\<^sub>f right_cart_proj \<nat>\<^sub>c (\<nat>\<^sub>c\<^bsup>(\<nat>\<^sub>c \<times>\<^sub>c \<nat>\<^sub>c\<^bsup>\<nat>\<^sub>c\<^esup>)\<^esup>))
+                                                       \<circ>\<^sub>c (id (\<nat>\<^sub>c \<times>\<^sub>c (\<nat>\<^sub>c\<^bsup>\<nat>\<^sub>c\<^esup>)) \<times>\<^sub>f    indexed_sum1) \<circ>\<^sub>c \<langle>\<langle>a,f\<rangle>, zero\<rangle>) +\<^sub>\<nat> 
+                      ((eval_func \<nat>\<^sub>c (\<nat>\<^sub>c \<times>\<^sub>c \<nat>\<^sub>c\<^bsup>\<nat>\<^sub>c\<^esup>)) \<circ>\<^sub>c (id (\<nat>\<^sub>c \<times>\<^sub>c (\<nat>\<^sub>c\<^bsup>\<nat>\<^sub>c\<^esup>)) \<times>\<^sub>f right_cart_proj \<nat>\<^sub>c (\<nat>\<^sub>c\<^bsup>(\<nat>\<^sub>c \<times>\<^sub>c \<nat>\<^sub>c\<^bsup>\<nat>\<^sub>c\<^esup>)\<^esup>))
+                                                       \<circ>\<^sub>c (id (\<nat>\<^sub>c \<times>\<^sub>c (\<nat>\<^sub>c\<^bsup>\<nat>\<^sub>c\<^esup>)) \<times>\<^sub>f    indexed_sum1) \<circ>\<^sub>c \<langle>\<langle>a,g\<rangle>, zero\<rangle>)" 
+      using assms by (typecheck_cfuncs,simp add: comp_associative2 identity_distributes_across_composition)
+    also have "... =  ((eval_func \<nat>\<^sub>c (\<nat>\<^sub>c \<times>\<^sub>c \<nat>\<^sub>c\<^bsup>\<nat>\<^sub>c\<^esup>)) \<circ>\<^sub>c (id (\<nat>\<^sub>c \<times>\<^sub>c (\<nat>\<^sub>c\<^bsup>\<nat>\<^sub>c\<^esup>)) \<times>\<^sub>f right_cart_proj \<nat>\<^sub>c (\<nat>\<^sub>c\<^bsup>(\<nat>\<^sub>c \<times>\<^sub>c \<nat>\<^sub>c\<^bsup>\<nat>\<^sub>c\<^esup>)\<^esup>))
+                                                       \<circ>\<^sub>c \<langle>\<langle>a,f\<rangle>, \<langle>zero, (eval_func \<nat>\<^sub>c \<nat>\<^sub>c \<circ>\<^sub>c left_cart_proj (\<nat>\<^sub>c \<times>\<^sub>c \<nat>\<^sub>c\<^bsup>\<nat>\<^sub>c\<^esup>) one)\<^sup>\<sharp>\<rangle>\<rangle>) +\<^sub>\<nat> 
+                      ((eval_func \<nat>\<^sub>c (\<nat>\<^sub>c \<times>\<^sub>c \<nat>\<^sub>c\<^bsup>\<nat>\<^sub>c\<^esup>)) \<circ>\<^sub>c (id (\<nat>\<^sub>c \<times>\<^sub>c (\<nat>\<^sub>c\<^bsup>\<nat>\<^sub>c\<^esup>)) \<times>\<^sub>f right_cart_proj \<nat>\<^sub>c (\<nat>\<^sub>c\<^bsup>(\<nat>\<^sub>c \<times>\<^sub>c \<nat>\<^sub>c\<^bsup>\<nat>\<^sub>c\<^esup>)\<^esup>))
+                                                       \<circ>\<^sub>c \<langle>\<langle>a,g\<rangle>, \<langle>zero, (eval_func \<nat>\<^sub>c \<nat>\<^sub>c \<circ>\<^sub>c left_cart_proj (\<nat>\<^sub>c \<times>\<^sub>c \<nat>\<^sub>c\<^bsup>\<nat>\<^sub>c\<^esup>) one)\<^sup>\<sharp>\<rangle>\<rangle>)" 
+      using assms by (typecheck_cfuncs, simp add: cfunc_cross_prod_comp_cfunc_prod id_left_unit2 indexed_sum1_zero)
+    also have "... =  ((eval_func \<nat>\<^sub>c (\<nat>\<^sub>c \<times>\<^sub>c \<nat>\<^sub>c\<^bsup>\<nat>\<^sub>c\<^esup>)) \<circ>\<^sub>c \<langle>\<langle>a,f\<rangle>, (eval_func \<nat>\<^sub>c \<nat>\<^sub>c \<circ>\<^sub>c left_cart_proj (\<nat>\<^sub>c \<times>\<^sub>c \<nat>\<^sub>c\<^bsup>\<nat>\<^sub>c\<^esup>) one)\<^sup>\<sharp>\<rangle>) +\<^sub>\<nat> 
+                      ((eval_func \<nat>\<^sub>c (\<nat>\<^sub>c \<times>\<^sub>c \<nat>\<^sub>c\<^bsup>\<nat>\<^sub>c\<^esup>)) \<circ>\<^sub>c \<langle>\<langle>a,g\<rangle>, (eval_func \<nat>\<^sub>c \<nat>\<^sub>c \<circ>\<^sub>c left_cart_proj (\<nat>\<^sub>c \<times>\<^sub>c \<nat>\<^sub>c\<^bsup>\<nat>\<^sub>c\<^esup>) one)\<^sup>\<sharp>\<rangle>)" 
+      using assms by (typecheck_cfuncs, simp add: cfunc_cross_prod_comp_cfunc_prod id_left_unit2 right_cart_proj_cfunc_prod)
+*)
+
+    have "((right_cart_proj \<nat>\<^sub>c (\<nat>\<^sub>c\<^bsup>(\<nat>\<^sub>c \<times>\<^sub>c \<nat>\<^sub>c\<^bsup>\<nat>\<^sub>c\<^esup>)\<^esup>) \<circ>\<^sub>c indexed_sum1)\<^sup>\<flat> \<circ>\<^sub>c
+     \<langle>\<langle>a,(add2 \<circ>\<^sub>c (eval_func \<nat>\<^sub>c \<nat>\<^sub>c \<times>\<^sub>f eval_func \<nat>\<^sub>c \<nat>\<^sub>c) \<circ>\<^sub>c distribute_left \<nat>\<^sub>c (\<nat>\<^sub>c\<^bsup>\<nat>\<^sub>c\<^esup>) (\<nat>\<^sub>c\<^bsup>\<nat>\<^sub>c\<^esup>))\<^sup>\<sharp> \<circ>\<^sub>c \<langle>f,g\<rangle>\<rangle> \<circ>\<^sub>c \<beta>\<^bsub>\<nat>\<^sub>c\<^esub>,id\<^sub>c \<nat>\<^sub>c\<rangle>) \<circ>\<^sub>c zero =
+    (right_cart_proj \<nat>\<^sub>c (\<nat>\<^sub>c\<^bsup>(\<nat>\<^sub>c \<times>\<^sub>c \<nat>\<^sub>c\<^bsup>\<nat>\<^sub>c\<^esup>)\<^esup>) \<circ>\<^sub>c indexed_sum1)\<^sup>\<flat> \<circ>\<^sub>c
+     \<langle>\<langle>a,(add2 \<circ>\<^sub>c (eval_func \<nat>\<^sub>c \<nat>\<^sub>c \<times>\<^sub>f eval_func \<nat>\<^sub>c \<nat>\<^sub>c) \<circ>\<^sub>c distribute_left \<nat>\<^sub>c (\<nat>\<^sub>c\<^bsup>\<nat>\<^sub>c\<^esup>) (\<nat>\<^sub>c\<^bsup>\<nat>\<^sub>c\<^esup>))\<^sup>\<sharp> \<circ>\<^sub>c \<langle>f,g\<rangle>\<rangle>,zero\<rangle>" 
+      using assms by (etcs_assocr,typecheck_cfuncs, metis cart_prod_extract_right)
+    also have "... = (eval_func \<nat>\<^sub>c (\<nat>\<^sub>c \<times>\<^sub>c \<nat>\<^sub>c\<^bsup>\<nat>\<^sub>c\<^esup>)) \<circ>\<^sub>c (id (\<nat>\<^sub>c \<times>\<^sub>c (\<nat>\<^sub>c\<^bsup>\<nat>\<^sub>c\<^esup>)) \<times>\<^sub>f ((right_cart_proj \<nat>\<^sub>c (\<nat>\<^sub>c\<^bsup>(\<nat>\<^sub>c \<times>\<^sub>c \<nat>\<^sub>c\<^bsup>\<nat>\<^sub>c\<^esup>)\<^esup>)) \<circ>\<^sub>c indexed_sum1)) \<circ>\<^sub>c
+     \<langle>\<langle>a,(add2 \<circ>\<^sub>c (eval_func \<nat>\<^sub>c \<nat>\<^sub>c \<times>\<^sub>f eval_func \<nat>\<^sub>c \<nat>\<^sub>c) \<circ>\<^sub>c distribute_left \<nat>\<^sub>c (\<nat>\<^sub>c\<^bsup>\<nat>\<^sub>c\<^esup>) (\<nat>\<^sub>c\<^bsup>\<nat>\<^sub>c\<^esup>))\<^sup>\<sharp> \<circ>\<^sub>c \<langle>f,g\<rangle>\<rangle>,zero\<rangle>" 
+      using assms comp_associative2 inv_transpose_func_def2 by (typecheck_cfuncs, auto)
+    also have "... = (eval_func \<nat>\<^sub>c (\<nat>\<^sub>c \<times>\<^sub>c \<nat>\<^sub>c\<^bsup>\<nat>\<^sub>c\<^esup>)) \<circ>\<^sub>c (id (\<nat>\<^sub>c \<times>\<^sub>c (\<nat>\<^sub>c\<^bsup>\<nat>\<^sub>c\<^esup>)) \<times>\<^sub>f (right_cart_proj \<nat>\<^sub>c (\<nat>\<^sub>c\<^bsup>(\<nat>\<^sub>c \<times>\<^sub>c \<nat>\<^sub>c\<^bsup>\<nat>\<^sub>c\<^esup>)\<^esup>))) \<circ>\<^sub>c 
+                                                        (id (\<nat>\<^sub>c \<times>\<^sub>c (\<nat>\<^sub>c\<^bsup>\<nat>\<^sub>c\<^esup>)) \<times>\<^sub>f indexed_sum1) \<circ>\<^sub>c
+     \<langle>\<langle>a,(add2 \<circ>\<^sub>c (eval_func \<nat>\<^sub>c \<nat>\<^sub>c \<times>\<^sub>f eval_func \<nat>\<^sub>c \<nat>\<^sub>c) \<circ>\<^sub>c distribute_left \<nat>\<^sub>c (\<nat>\<^sub>c\<^bsup>\<nat>\<^sub>c\<^esup>) (\<nat>\<^sub>c\<^bsup>\<nat>\<^sub>c\<^esup>))\<^sup>\<sharp> \<circ>\<^sub>c \<langle>f,g\<rangle>\<rangle>,zero\<rangle>" 
+      using assms by (typecheck_cfuncs, simp add: comp_associative2 identity_distributes_across_composition)
+    also have "... = (eval_func \<nat>\<^sub>c (\<nat>\<^sub>c \<times>\<^sub>c \<nat>\<^sub>c\<^bsup>\<nat>\<^sub>c\<^esup>)) \<circ>\<^sub>c (id (\<nat>\<^sub>c \<times>\<^sub>c (\<nat>\<^sub>c\<^bsup>\<nat>\<^sub>c\<^esup>)) \<times>\<^sub>f (right_cart_proj \<nat>\<^sub>c (\<nat>\<^sub>c\<^bsup>(\<nat>\<^sub>c \<times>\<^sub>c \<nat>\<^sub>c\<^bsup>\<nat>\<^sub>c\<^esup>)\<^esup>))) \<circ>\<^sub>c                                                        
+     \<langle>\<langle>a,(add2 \<circ>\<^sub>c (eval_func \<nat>\<^sub>c \<nat>\<^sub>c \<times>\<^sub>f eval_func \<nat>\<^sub>c \<nat>\<^sub>c) \<circ>\<^sub>c distribute_left \<nat>\<^sub>c (\<nat>\<^sub>c\<^bsup>\<nat>\<^sub>c\<^esup>) (\<nat>\<^sub>c\<^bsup>\<nat>\<^sub>c\<^esup>))\<^sup>\<sharp> \<circ>\<^sub>c \<langle>f,g\<rangle>\<rangle>,
+     \<langle>zero, (eval_func \<nat>\<^sub>c \<nat>\<^sub>c \<circ>\<^sub>c left_cart_proj (\<nat>\<^sub>c \<times>\<^sub>c \<nat>\<^sub>c\<^bsup>\<nat>\<^sub>c\<^esup>) one)\<^sup>\<sharp>\<rangle>\<rangle>" 
+      using assms by(typecheck_cfuncs, smt (verit, best) cfunc_cross_prod_comp_cfunc_prod comp_associative2 id_left_unit2 indexed_sum1_zero)
+ 
 
 
 
+
+(* 
+*)
+
+(*
+  have "indexed_sum \<circ>\<^sub>c \<langle>\<langle>a, meta_add \<nat>\<^sub>c \<circ>\<^sub>c \<langle>f, g\<rangle>\<rangle> \<circ>\<^sub>c \<beta>\<^bsub>\<nat>\<^sub>c\<^esub>, id \<nat>\<^sub>c\<rangle> = 
+        add2 \<circ>\<^sub>c \<langle>indexed_sum \<circ>\<^sub>c \<langle>\<langle>a, f\<rangle> \<circ>\<^sub>c \<beta>\<^bsub>\<nat>\<^sub>c\<^esub>, id \<nat>\<^sub>c\<rangle>, indexed_sum \<circ>\<^sub>c \<langle>\<langle>a, g\<rangle>\<circ>\<^sub>c \<beta>\<^bsub>\<nat>\<^sub>c\<^esub>, id \<nat>\<^sub>c\<rangle>\<rangle>"
+  proof(rule natural_number_object_func_unique[where X = "\<nat>\<^sub>c"])
+    show "indexed_sum \<circ>\<^sub>c \<langle>\<langle>a,meta_add \<nat>\<^sub>c \<circ>\<^sub>c \<langle>f,g\<rangle>\<rangle> \<circ>\<^sub>c \<beta>\<^bsub>\<nat>\<^sub>c\<^esub>,id\<^sub>c \<nat>\<^sub>c\<rangle> : \<nat>\<^sub>c \<rightarrow> \<nat>\<^sub>c"
+      using assms by typecheck_cfuncs
+    show "add2 \<circ>\<^sub>c \<langle>indexed_sum \<circ>\<^sub>c \<langle>\<langle>a,f\<rangle> \<circ>\<^sub>c \<beta>\<^bsub>\<nat>\<^sub>c\<^esub>,id\<^sub>c \<nat>\<^sub>c\<rangle>,indexed_sum \<circ>\<^sub>c \<langle>\<langle>a,g\<rangle> \<circ>\<^sub>c \<beta>\<^bsub>\<nat>\<^sub>c\<^esub>,id\<^sub>c \<nat>\<^sub>c\<rangle>\<rangle> : \<nat>\<^sub>c \<rightarrow> \<nat>\<^sub>c"
+      using assms by typecheck_cfuncs
+  next
+    have "(indexed_sum \<circ>\<^sub>c \<langle>\<langle>a,meta_add \<nat>\<^sub>c \<circ>\<^sub>c \<langle>f,g\<rangle>\<rangle> \<circ>\<^sub>c \<beta>\<^bsub>\<nat>\<^sub>c\<^esub>,id\<^sub>c \<nat>\<^sub>c\<rangle>) \<circ>\<^sub>c zero = 
+           indexed_sum \<circ>\<^sub>c \<langle>\<langle>a,meta_add \<nat>\<^sub>c \<circ>\<^sub>c \<langle>f,g\<rangle>\<rangle>,zero\<rangle>"
+      using assms by(etcs_assocr,typecheck_cfuncs, metis cart_prod_extract_right)
+    also have "... =  cnufatem (meta_add \<nat>\<^sub>c \<circ>\<^sub>c \<langle>f,g\<rangle>) \<circ>\<^sub>c a"
+      using assms indexed_sum_uppr_eq_lwr by (typecheck_cfuncs, presburger)
+    also have "... = (cnufatem (f) \<circ>\<^sub>c a) +\<^sub>\<nat>  (cnufatem (g) \<circ>\<^sub>c a) "
+      using assms apply typecheck_cfuncs
+*)
+
+
+
+
+
+(Use meta_add below)
+lemma indexed_sum_split:
+  assumes "a \<in>\<^sub>c \<nat>\<^sub>c"
+  assumes "m \<in>\<^sub>c \<nat>\<^sub>c"
+  assumes "q \<in>\<^sub>c \<nat>\<^sub>c"
+  assumes "n = (successor \<circ>\<^sub>c m) +\<^sub>\<nat> q"
+  assumes "f \<in>\<^sub>c \<nat>\<^sub>c\<^bsup>\<nat>\<^sub>c\<^esup>"
+  shows "indexed_sum \<circ>\<^sub>c \<langle>\<langle>a, f\<rangle>, n \<rangle> =   indexed_sum \<circ>\<^sub>c \<langle>\<langle>a, f\<rangle>, m\<rangle> +\<^sub>\<nat> indexed_sum \<circ>\<^sub>c \<langle>\<langle>a +\<^sub>\<nat> (successor \<circ>\<^sub>c m), f\<rangle>, q\<rangle>"
+proof(unfold indexed_sum_def)
+  have n_type[type_rule]: "n \<in>\<^sub>c \<nat>\<^sub>c"
+    using assms(2-4) by (simp add: add_type succ_n_type)
+  have "(right_cart_proj \<nat>\<^sub>c (\<nat>\<^sub>c\<^bsup>(\<nat>\<^sub>c \<times>\<^sub>c \<nat>\<^sub>c\<^bsup>\<nat>\<^sub>c\<^esup>)\<^esup>) \<circ>\<^sub>c indexed_sum1)\<^sup>\<flat> \<circ>\<^sub>c \<langle>\<langle>a,f\<rangle>,n\<rangle> =
+        (eval_func  \<nat>\<^sub>c (\<nat>\<^sub>c \<times>\<^sub>c \<nat>\<^sub>c\<^bsup>\<nat>\<^sub>c\<^esup>)
+               \<circ>\<^sub>c (id(\<nat>\<^sub>c \<times>\<^sub>c \<nat>\<^sub>c\<^bsup>\<nat>\<^sub>c\<^esup>) \<times>\<^sub>f (right_cart_proj \<nat>\<^sub>c (\<nat>\<^sub>c\<^bsup>(\<nat>\<^sub>c \<times>\<^sub>c \<nat>\<^sub>c\<^bsup>\<nat>\<^sub>c\<^esup>)\<^esup>)  \<circ>\<^sub>c indexed_sum1) )) \<circ>\<^sub>c \<langle>\<langle>a,f\<rangle>,n\<rangle>"
+    by (typecheck_cfuncs, simp add: comp_associative2 inv_transpose_func_def2)
+  also have "... =
 
 (*
 definition indexed_sum :: "cfunc \<Rightarrow> cfunc \<Rightarrow> cfunc" where
